Fix address collision semantics
Although it is not clear to me whether https://eips.ethereum.org/EIPS/eip-7610 is part of Cancun or not, it
seems that the tests all expect it to be in force, so we implement it to pass them.

vfmExecutionScript.sml
@@ -11,6 +11,10 @@ Definition update_storage_def:
   update_storage k v (s: storage) = (k =+ v) s
 End
 
+Definition storage_empty_def:
+  storage_empty (s: storage) = (s = empty_storage)
+End
+
 Definition b2w_def[simp]:
   b2w T = 1w ∧ b2w F = 0w
 End
@@ -29,12 +33,13 @@ Definition sign_extend_def:
     word_of_bytes T 0w $ REPLICATE m sw ++ bs
 End
 
-Definition account_has_code_or_nonce_def:
-  account_has_code_or_nonce a = ¬(a.nonce = 0 ∧ NULL a.code)
+Definition account_already_created_def:
+  account_already_created a =
+    ¬(a.nonce = 0 ∧ NULL a.code ∧ storage_empty a.storage)
 End
 
 Definition account_empty_def:
-  account_empty a ⇔ a.balance = 0 ∧ ¬account_has_code_or_nonce a
+  account_empty a ⇔ a.balance = 0 ∧ a.nonce = 0 ∧ NULL a.code
 End
 
 Definition memory_cost_def:
@@ -965,7 +970,7 @@ Definition step_create_def:
        SUC nonce ≥ 2 ** 64 ∨
        sucDepth > 1024
     then abort_unuse cappedGas
-    else if account_has_code_or_nonce toCreate
+    else if account_already_created toCreate
     then abort_create_exists senderAddress sender
     else proceed_create senderAddress sender
            address value code toCreate cappedGas
@@ -1344,7 +1349,7 @@ Definition run_create_def:
              transfer_value tx.from calleeAddress tx.value)
     else
       let callee = lookup_account calleeAddress s.accounts in
-      if account_has_code_or_nonce callee then
+      if account_already_created callee then
         INL $ post_transaction_accounting blk tx (SOME AddressCollision) s.accounts
               (s with contexts := [ctxt with gasUsed := ctxt.callParams.gasLimit])
       else
